wip: edsl v2, now should do the right thing

SSA/Projects/Tensor2D/Tensor2D.lean
@@ -5,20 +5,20 @@ import SSA.Core.Util
 
 
 /-- Tensor2d with existential dimension sizes. -/
-structure Tensor2d' (α : Type) where 
+structure Tensor2d' (α : Type) where
   n₀ : ℕ
   n₁ : ℕ
   mat : Matrix (Fin n₀) (Fin n₁) α
 
 
-def Tensor2d'.transpose (t : Tensor2d' α) : Tensor2d' α where 
+def Tensor2d'.transpose (t : Tensor2d' α) : Tensor2d' α where
   n₀ := t.n₁
-  n₁ := t.n₀  
+  n₁ := t.n₀
   mat := t.mat.transpose
 
 theorem Tensor2d'.transpose_transpose (t : Tensor2d' α) : t.transpose.transpose = t := rfl
 
-def Tensor2d'.map (f : α → β) (t : Tensor2d' α) : Tensor2d' β where 
+def Tensor2d'.map (f : α → β) (t : Tensor2d' α) : Tensor2d' β where
   n₀ := t.n₀
   n₁ := t.n₁
   mat := t.mat.map f
@@ -32,16 +32,16 @@ def const (a : α) (_b : β) : α := a
 def Tensor2d'.fill (v : β) (t : Tensor2d' α) : Tensor2d' β := t.map (const v)
 
 /-- extract a submatrix of (sz₀ × sz₁) size at offset (δ₀, δ₁). Fails if this is out of bounds. -/
-def Tensor2d'.extract (δ₀ δ₁ : ℕ) (sz₀ sz₁ : ℕ) (t : Tensor2d' α) : Option (Tensor2d' α) := 
-  if SZ0 : δ₀ + sz₀ ≤ t.n₀ then 
-    if SZ1 : δ₁ + sz₁ ≤ t.n₁ then 
+def Tensor2d'.extract (δ₀ δ₁ : ℕ) (sz₀ sz₁ : ℕ) (t : Tensor2d' α) : Option (Tensor2d' α) :=
+  if SZ0 : δ₀ + sz₀ ≤ t.n₀ then
+    if SZ1 : δ₁ + sz₁ ≤ t.n₁ then
       {
         n₀ := sz₀,
         n₁ := sz₁,
-        mat := Matrix.of fun (ix₀ : Fin sz₀) (ix₁ : Fin sz₁) => 
-          have INBOUNDS0 : δ₀ + ix₀ < t.n₀ := by linarith[ix₀.isLt] 
-          have INBOUNDS1 : δ₁ + ix₁ < t.n₁ := by linarith[ix₁.isLt] 
-          t.mat ⟨δ₀ + ix₀, INBOUNDS0⟩ ⟨δ₁ + ix₁, INBOUNDS1⟩   
+        mat := Matrix.of fun (ix₀ : Fin sz₀) (ix₁ : Fin sz₁) =>
+          have INBOUNDS0 : δ₀ + ix₀ < t.n₀ := by linarith[ix₀.isLt]
+          have INBOUNDS1 : δ₁ + ix₁ < t.n₁ := by linarith[ix₁.isLt]
+          t.mat ⟨δ₀ + ix₀, INBOUNDS0⟩ ⟨δ₁ + ix₁, INBOUNDS1⟩
         : Tensor2d' α
       }
     else none
@@ -65,3 +65,92 @@ theorem Tensor2d'.fill_extract (δ₀ δ₁ sz₀ sz₁ : ℕ) (t : Tensor2d' α
   (t.fill v).extract δ₀ δ₁ sz₀ sz₁ = (t.extract δ₀ δ₁ sz₀ sz₁).map (Tensor2d'.fill v) := by {
     simp only[fill, Tensor2d'.map_extract]
 }
+
+
+inductive Op
+| add
+| const (v: Nat)
+| sub
+
+inductive BaseType
+| int : BaseType
+| nat : BaseType
+deriving DecidableEq, Inhabited
+
+instance : Goedel BaseType where
+  toType
+  | .int => Int
+  | .nat => Nat
+
+
+abbrev UserType := SSA.UserType BaseType
+
+-- Can we get rid of the code repetition here? (not that copilot has any trouble completing this)
+@[simp]
+def argUserType : Op → UserType
+| Op.add => .pair (.base BaseType.int) (.base BaseType.int)
+| Op.sub => .pair (.base BaseType.int) (.base BaseType.int)
+| Op.const _ => .unit
+
+@[simp]
+def outUserType : Op → UserType
+| Op.add => .base (BaseType.int)
+| Op.sub => .base (BaseType.int)
+| Op.const _ => .base (BaseType.nat)
+
+@[simp]
+def rgnDom : Op → UserType
+| Op.add => .unit
+| Op.sub => .unit
+| Op.const _ => .unit
+
+@[simp]
+def rgnCod : Op → UserType
+| Op.add => .unit
+| Op.sub => .unit
+| Op.const _ => .unit
+
+def eval (o : Op)
+  (arg: Goedel.toType (argUserType o))
+  (_rgn : (Goedel.toType (rgnDom o) → (Goedel.toType (rgnCod o)))) :
+  (Goedel.toType (outUserType o)) :=
+  match o with
+  | .const v => v
+  | .add =>
+    let (x, y) := arg;
+    let x : Int := x;
+    let y : Int := y;
+    x + y
+  | .sub =>
+    let (x, y) := arg;
+    let x : Int := x;
+    let y : Int := y;
+    x - y
+
+instance TUS : SSA.TypedUserSemantics Op BaseType where
+  argUserType := argUserType
+  rgnDom := rgnDom
+  rgnCod := rgnCod
+  outUserType := outUserType
+  eval := eval
+
+syntax "map1d" : dsl_op
+syntax "extract1d" : dsl_op
+syntax "const" "(" term ")" : dsl_op
+
+open EDSL in
+macro_rules
+| `([dsl_op| map1d]) => `(Op.map1d)
+| `([dsl_op| extract1d]) => `(Op.extract1d)
+| `([dsl_op| const ($x)]) => `(Op.const $x) -- note that we use the syntax extension to enrich the base DSL
+
+
+
+open SSA EDSL2 in
+theorem map_functorial_edsl :
+  TSSA.eval (e := e) (Op := Op) (β := BaseType) [dsl_bb2|
+    return ()
+  ] =
+  TSSA.eval (e := e) (Op := Op) (β := BaseType) [dsl_bb2|
+    return ()
+  ] := sorry
